$$
\begin{align}
(1+x+x^2+x^3+\dots)&=\frac 1 {1-x}\\
(1+x^2+x^4+x^6+\dots)&=\frac 1 {1-x^2}\\
\end{align}
$$




$$
(1+x+x^2+x^3+x^4)=\frac{1-x^5}{1-x}
$$

$$
\begin{align}
数论a 为等比数列,首项 a_1 公比q\\
\sum\limits_{i=1}^na_i=\frac {a_1(1-q^n) }{1-q}
\end {align}
$$
$$
\begin{align}
(a+b)^n&=\sum\limits^n_{k=0}\binom{n}{k}a^kb^{n-k}\\
\binom{n}{k}&=\frac {P^k_n} {k!}=\frac{k!}{k!(n-k)!}\\
(1+x)^n&=\sum\limits^\infty_{k=0}\binom{n}{k}x^k\\
\frac 1 {(1-x)^n}&=\sum\limits^\infty_{k=0}\binom{n+k-1}{k}x^k\\\
e^x&=\sum\limits_{i=0}^\infty\frac 1{i!}x^i
\end{align}
$$

